Cdclt/Lift/Coe.lean
@@ -7,10 +7,10 @@ open proof
 open sort
 open term
 
-instance {Δ : SEnvironment} : Coe (interpSort Δ (atom 1)) Bool where
+instance {Δ : SEnvironment} : Coe (interpSort Δ (atom 1)) Prop where
   coe e := e
 
-instance {Δ : SEnvironment} : Coe (interpSort Δ boolSort) Bool where
+instance {Δ : SEnvironment} : Coe (interpSort Δ boolSort) Prop where
   coe e := e
 
 def coe' : (A = B) → A → B
