Cdclt/Lift/Env.lean
@@ -15,19 +15,12 @@ def defaultValue (Δ : SEnvironment) (s : sort) : interpSort Δ s :=
   match s with
   | arrow s₁ s₂ => λ _ => defaultValue Δ s₂
   | atom 0 => Sigma.snd (Δ 0)
-  | atom 1 => false
+  | atom 1 => False
   | atom (succ (succ i)) => Sigma.snd (Δ (succ (succ i)))
-  | sort.undef => false
-  | sort.array _ _ => false
-  | sort.bv _ => false
-  | sort.dep => false
+  | sort.undef => False
+  | sort.array _ _ => False
+  | sort.bv _ => False
+  | sort.dep => False
 
 def defaultEnvironment: Environment := λ _ Δ s => defaultValue Δ s
 
-
-/- def extendEnv (i : Nat) (Δ : SEnvironment) (s : sort) (a : interpSort Δ s) (Γ : Environment) : Environment := -/
-/-   λ j Δ' s' => if j == i -/
-/-                then if r: Δ = Δ' -/
-/-                     then coe' (congrArg (interpSort Δ') r) a -/
-/-                     else Γ j s' -/
-/-            else Γ j s' -/
