Cdclt/Lift/Types.lean
@@ -12,11 +12,9 @@ def SEnvironment : Type 1 := Nat → (Σ (A : Type) , A)
 def interpSort (Δ : SEnvironment) (s : sort) : Type :=
   match s with
   | sort.arrow s₁ s₂ => (interpSort Δ s₁) → (interpSort Δ s₂)
-  | sort.atom 1 => Bool
+  | sort.atom 1 => Prop
   | sort.atom n => Sigma.fst (Δ n)
-  | _ => Bool
-
-#check interpSort
+  | _ => Prop
 
 -- takes the number of a constant and it's type, and returns its value
 def Environment : Type 1 := Nat → (Δ : SEnvironment) → (s : sort) → interpSort Δ s
